theories/sim/global_adequacy.v
@@ -1,0 +1,143 @@
+From Coq Require Import Program.Equality Lia.
+From Paco Require Import paco.
+
+From stbor.lang Require Import steps_wf.
+From stbor.sim Require Import global invariant sflib.
+
+Set Default Proof Using "Type".
+
+(** Behaviors ----------------------------------------------------------------*)
+
+Section BEHAVIOR.
+  Context {Config State Value: Type}
+           (step: forall (conf:Config) (s s':State), Prop)
+           (term: forall (conf:Config) (s:State) (val:Value), Prop)
+  .
+
+  Inductive observation: Type :=
+  | obs_term (retval:Value)
+  | obs_inftau
+  .
+
+  Inductive behmatch
+            (conf:Config)
+            (behave: forall (s:State) (obs:observation), Prop)
+    : forall (s:State) (obs:observation), Prop :=
+  | beh_stuck
+      s obs
+      (NT: forall val, ¬ term conf s val)
+      (NS: ∀ s', ¬ step conf s s')
+    : behmatch conf behave s obs
+  | beh_term
+      s v
+      (TERM: term conf s v)
+    : behmatch conf behave s (obs_term v)
+  | beh_inftau
+      s s'
+      (STEP: step conf s s')
+      (INF: behave s' obs_inftau)
+    : behmatch conf behave s obs_inftau
+  .
+  Hint Constructors behmatch.
+
+  Inductive behave_ (conf:Config) behave (s:State) (obs:observation): Prop :=
+  | behave_intro
+      s'
+      (TAU: rtc (step conf) s s')
+      (MAT: behmatch conf behave s' obs)
+  .
+  Hint Constructors behave_.
+
+  Lemma behave_mon conf: monotone2 (behave_ conf).
+  Proof.
+    repeat intro. destruct IN. destruct MAT; eauto.
+  Qed.
+  Hint Resolve behave_mon: paco.
+
+  Definition behave (conf:Config): forall (s:State) (obs:observation), Prop := paco2 (behave_ conf) bot2.
+End BEHAVIOR.
+Hint Constructors behmatch.
+Hint Constructors behave_.
+Hint Resolve behave_mon: paco.
+
+Definition init_expr := (Call #["main"] []).
+Definition init_state := (mkState ∅ ∅ [] O O).
+
+Definition term (prog:fn_env) (s:expr * state) (v:value): Prop :=
+  to_result s.1 = Some (ValR v).
+
+Definition behave_prog (prog:fn_env) (obs:@observation value): Prop :=
+  behave tstep term prog (init_expr, init_state) obs.
+
+(* TODO: move *)
+Lemma tc_inv_l
+      A (R:relation A) x z
+      (TC: tc R x z):
+  exists y, rtc R x y /\ R y z.
+Proof.
+  induction TC.
+  - esplits; eauto. reflexivity.
+  - des. esplits; [|by eauto]. eapply rtc_l; eauto.
+Qed.
+
+(* TODO: move *)
+Lemma strong_induction
+      (P : nat -> Prop)
+      (IH: forall (n:nat) (IH: forall (k:nat) (LT: (k < n)%nat), P k), P n):
+  forall n : nat, P n.
+Proof.
+  i. cut (forall (m k:nat), (k < m -> P k)%nat); [by eauto|].
+  induction m.
+  - i. nia.
+  - i. apply lt_le_S in H. inv H; eauto.
+Qed.
+
+Lemma adequacy
+      prog_src prog_tgt idx conf_src conf_tgt
+      (SIM: sim prog_src prog_tgt idx conf_src conf_tgt)
+  : behave tstep term prog_tgt conf_tgt <1= behave tstep term prog_src conf_src.
+Proof.
+  revert idx conf_src conf_tgt SIM. pcofix CIH. intros.
+  punfold PR. inv PR.
+  rename x2 into obs. rename s' into conf'_tgt. revert idx conf_src SIM MAT.
+  dependent induction TAU; cycle 1.
+  - rename x into conf_tgt.
+    rename y into conf'_tgt.
+    rename z into conf''_tgt.
+    i. punfold SIM. exploit SIM.
+    { admit. (* WF *) }
+    { admit. (* WF *) }
+    clear SIM. intro SIM. inv SIM.
+    exploit sim_step; eauto. i. des.
+    + inv x0; ss.
+      rename eσ2_src into conf'_src.
+      exploit IHTAU; eauto.
+      intro BEH. punfold BEH. inv BEH.
+      pfold. econs; [|by eauto]. etrans; eauto. apply tc_rtc. ss.
+    + inv x0; ss.
+      rename eσ2_src into conf'_src.
+      exploit IHTAU; eauto.
+  - intros idx. revert x.
+    induction idx using strong_induction. i.
+    punfold SIM. exploit SIM.
+    { admit. (* WF *) }
+    { admit. (* WF *) }
+    clear SIM. intro SIM. inv SIM. inv MAT.
+    + exploit sim_stuck; eauto.
+      { admit. (* property of stuck *) }
+      i. des.
+      pfold. econs; eauto.
+      admit. (* property of stuck *)
+    + exploit sim_terminal; eauto. i. des.
+      pfold. econs; eauto.
+      econs 2.
+      admit. (* property of terminal *)
+    + pclearbot. exploit sim_step; eauto. i. des.
+      * inv x1; ss.
+        exploit CIH; eauto. i.
+        apply tc_inv_l in x0. des.
+        pfold. econs; eauto.
+      * inv x1; ss. exploit IH; eauto.
+        punfold INF. inv INF. inv TAU; eauto.
+        econs 3; eauto.
+Admitted.
