theories/sim/local_adequacy.v
@@ -1,0 +1,7 @@
+From Coq Require Import Program.Equality Lia.
+From Paco Require Import paco.
+
+From stbor.lang Require Import steps_wf.
+From stbor.sim Require Import global invariant sflib.
+
+Set Default Proof Using "Type".
